Upd

Alphabet.v
@@ -1,36 +1,61 @@
-Require Import Arith.
+Require Import Arith List.
+Import ListNotations.
 
 Section Alphabet.
-  Definition at_least (n: nat) := { i: nat | i >= n }.
+  Record at_least (n: nat) := { atl_i :> nat; atl_prf: atl_i >= n }.
   Definition positive := at_least 1.
 
   Definition atl_to_nat {n: nat} (m: at_least n): nat.
     destruct m.
-    exact x.
+    exact atl_i0.
   Defined.
 
-  Definition nat_to_atl (n m: nat) {prf: m >= n}: at_least n.
-    exact (exist _ m prf).
-  Defined.
+  Definition nat_to_atl (n m: nat) (prf: m >= n): at_least n :=
+    {| atl_i := m; atl_prf := prf |}.
 
   Lemma pos_gt_zero (n: positive): 0 < atl_to_nat n.
   Proof.
-    simpl in *.
     unfold positive in n.
-    unfold at_least in n.
     destruct n.
-    simpl.
+    unfold atl_to_nat.
     auto.
   Qed.
 
-  Definition alphabet (n: positive) := { i: nat | i < atl_to_nat n }.
+  Record alphabet (n: positive) := { sym_i :> nat; sym_prf: sym_i < atl_to_nat n }.
 
-  Definition nat_to_alph (m: positive) (n: nat) (prf: n < atl_to_nat m): alphabet m.
-    exact (exist _ n prf).
+  Definition nat_to_sym (m: positive) (n: nat) (prf: n < atl_to_nat m): alphabet m :=
+    {| sym_i := n; sym_prf := prf |}.
+
+  Definition sym_to_nat {n: positive} (a: alphabet n): nat.
+    destruct a.
+    exact sym_i0.
   Defined.
 
-  Definition alph_to_nat {m: positive} (n: alphabet m): nat.
-    destruct n.
-    exact x.
+  Definition sym_0 (n: positive) := nat_to_sym n 0 (pos_gt_zero n).
+
+  Local Fixpoint all_syms' (n: positive) (i: nat) (prf: i < atl_to_nat n): list (alphabet n).
+    destruct i.
+    - exact (cons (nat_to_sym n 0 prf) nil).
+    - remember (nat_to_sym n (S i) prf) as m.
+      assert (prf' := prf).
+      apply Nat.lt_succ_l in prf'.
+      specialize all_syms' with n i.
+      exact (all_syms' prf' ++ [m]).
   Defined.
+
+  Definition all_syms (n: positive): list (alphabet n).
+    remember (Nat.lt_pred_l (atl_to_nat n)) as H.
+    remember (Nat.lt_neq 0 (atl_to_nat n) (pos_gt_zero n)) as Hn.
+    clear HeqHn.
+    apply Nat.neq_sym in Hn.
+    apply H in Hn.
+    exact (all_syms' n (Nat.pred (atl_to_nat n)) Hn).
+  Defined.
+
+  Lemma five_gt_one: 5 >= 1. Proof. auto 10. Qed.
+
+  Theorem sym_in_all_syms: forall (n: positive) (a: alphabet n), .
+  Proof.
+  Qed.
+
 End Alphabet.
